Geb/Prototypes/FreeTopos.lean
@@ -8,6 +8,7 @@ module
 public import Geb.Prototypes.FreeTopos.Arrows
 public import Geb.Prototypes.FreeTopos.Category
 public import Geb.Prototypes.FreeTopos.Check
+public import Geb.Prototypes.FreeTopos.Classifier
 public import Geb.Prototypes.FreeTopos.Infer
 public import Geb.Prototypes.FreeTopos.Internal
 public import Geb.Prototypes.FreeTopos.Model
